cleaned up composition

theories/prob_eff_lang/probblaze/examples/DH_KE/new_composition.v
@@ -30,13 +30,13 @@ Section new_comp_verification.
   Context `{!inG Σ (exclR unitO), !inG Σ dfracO,!inG Σ (dfrac_agreeR valO)}.
 
   Definition REAL_CHAN_DHKE : val :=
-    λ: "f", (F_OAUTH ||ₗ (λ: "f", F_AUTH (DH_KE "f"))%V) (CHAN "f").
+    λ: "f", ((λ: "f", F_AUTH (DH_KE "f"))%V ||ᵣ F_OAUTH) (CHAN "f").
 
   Definition REAL_CHAN_DH_REAL : val :=
-    λ: "f", (F_OAUTH ||ₗ (λ: "f", F_AUTH (C DH_real "f"))%V) (CHAN "f").
+    λ: "f", ( (λ: "f", F_AUTH (C DH_real "f"))%V ||ᵣ F_OAUTH) (CHAN "f").
 
   Definition REAL_CHAN_DH_RAND : val :=
-    λ: "f", (F_OAUTH ||ₗ (λ: "f", F_AUTH (C DH_rand "f")%V) (CHAN "f")).
+    λ: "f", ((λ: "f", F_AUTH (C DH_rand "f")%V ||ᵣ F_OAUTH) (CHAN "f")).
   
    (* F_OAUTH[ F_AUTH [DH_KE [CHAN []]]] ≤ F_OAUTH[ F_AUTH [C[DH_real][CHAN []]]] *)
   (*---------------------------------------------------------------------------*)
@@ -44,7 +44,7 @@ Section new_comp_verification.
     ⊢ sem_val_typed REAL_CHAN_DHKE REAL_CHAN_DH_REAL 
         (* the type should match the program. Look carefully at the order of the incoming effects *)
         (* the type of the client needs to change to a linear function *)
-        (∀ᵣ θ__L ,(∀ᵣ θₕ, (((⊤ × (sem_ty_sum 𝟙 𝟙)) -{ θₕ }-> (Option ⊤)) × ((sem_ty_sum 𝟙 𝟙) -{ θₕ }-> (Option  ⊤))) 
+        (∀ᵣ θ__L ,(∀ᵣ θₕ, (((⊤ × (sem_ty_sum 𝟙 𝟙)) -{ θₕ }-> 𝟙) × ((sem_ty_sum 𝟙 𝟙) -{ θₕ }-> (Option  ⊤))) 
                                                                    -{ sem_row_union  θₕ θ__L }-> 𝟙)
                   (* the product needs to be under a bang, since the effects can be used multiple times *)
                                                              ⊸ (∀ᵣ θ₁,∀ᵣ θ2, (((⊤ × (𝟙 + 𝟙)) -{ θ₁ }-> 𝟙) 
@@ -55,7 +55,7 @@ Section new_comp_verification.
     iApply func_comp_left.
     - admit.                    (* closed expressions *)
     - admit.                    (* closed expressions *)
-    - iIntros (θ). iApply brel_left_comp.
+    - iIntros (θ). iApply parallel_comp_right.
       + unfold τ__F. unshelve iApply F_AUTH_DH_KE_FAUTH_C_DH_real; try done. 
       + admit.                  (* F_OAUTH well-typed *)
     - admit.                    (* CHAN well-typed *)
@@ -82,53 +82,48 @@ Section new_comp_verification.
   Admitted.*)
 
   Lemma C_REAL_DHKE_F_OAUTH :
-     ⊢ sem_val_typed REAL_CHAN_DH_REAL REAL_CHAN_DHKE (∀ᵣ θ__L ,(∀ᵣ θₕ, (((⊤ × (sem_ty_sum 𝟙 𝟙)) -{ θₕ }-> (Option ⊤)) × ((sem_ty_sum 𝟙 𝟙) -{ θₕ }-> (Option  ⊤))) 
-                                                                   -{ sem_row_union  θₕ θ__L }-> 𝟙) 
-                                                             ⊸ (∀ᵣ θ₁,  (((⊤ × (𝟙 + 𝟙)) -{ θ₁ }-> 𝟙) × ((𝟙 + 𝟙) -{ θ₁ }-> Option ⊤)) 
-                                                                                 ⊸ ((𝟙 + 𝟙) -{ θ₁ }-> Option ⊤) -{ sem_row_union θ₁ θ__L }-∘ 𝟙))%T.
+     ⊢ sem_val_typed REAL_CHAN_DH_REAL REAL_CHAN_DHKE (∀ᵣ θ__L ,(∀ᵣ θₕ, (((⊤ × (sem_ty_sum 𝟙 𝟙)) -{ θₕ }-> 𝟙) × ((sem_ty_sum 𝟙 𝟙) -{ θₕ }-> (Option  ⊤))) 
+                                                                   -{ sem_row_union  θₕ θ__L }-> 𝟙)
+                                                             ⊸ (∀ᵣ θ₁,∀ᵣ θ2, (((⊤ × (𝟙 + 𝟙)) -{ θ₁ }-> 𝟙) 
+                                                                                 × ((𝟙 + 𝟙) -{ θ₁ }-> Option ⊤)) 
+                                                                                 ⊸ (((⊤ × (𝟙 + 𝟙)) -{ θ2 }-> 𝟙) 
+                                                                                 × ((𝟙 + 𝟙) -{ θ2 }-> Option ⊤)) -{ sem_row_union θ₁ (sem_row_union θ2 θ__L) }-∘ 𝟙))%T.
   Proof. 
     iApply func_comp_left.
     - admit.                    (* closed expressions *)
     - admit.                    (* closed expressions *)
-    - iIntros (θ). iApply brel_left_comp.
-      + unfold τ__F. About F_AUTH_DH_KE_FAUTH_C_DH_real.
-        iApply F_AUTH_C_DH_real_FAUTH_DH_KE; try done.
+    - iIntros (θ). iApply parallel_comp_right.
+      + unfold τ__F. iApply F_AUTH_C_DH_real_FAUTH_DH_KE; try done.
       + admit.                  (* F_OAUTH well-typed *)
     - admit.                    (* CHAN well-typed *)
   Admitted. 
 
   (*F_OAUTH [F_AUTH [C[DH_real][CHAN[]]]] ≤ F_OAUTH [F_AUTH [C[DH_rand][CHAN[]]]]*)
   (*-----------------------------------------------------------------------------*)
-  Lemma C_REAL_DH_RAND :
-    ⊢ sem_val_typed REAL_CHAN_DH_REAL REAL_CHAN_DH_RAND (∀ᵣ θ__L ,(∀ᵣ θₕ, (((⊤ × (sem_ty_sum 𝟙 𝟙)) -{ θₕ }-> (Option ⊤)) × ((sem_ty_sum 𝟙 𝟙) -{ θₕ }-> (Option  ⊤))) 
-                                                                   -{ sem_row_union  θₕ θ__L }-> 𝟙) 
-                                                             ⊸ (∀ᵣ θ₁,  (((⊤ × (𝟙 + 𝟙)) -{ θ₁ }-> 𝟙) × ((𝟙 + 𝟙) -{ θ₁ }-> Option ⊤)) 
-                                                                          ⊸ ((𝟙 + 𝟙) -{ θ₁ }-> Option ⊤) -{ sem_row_union θ₁ θ__L }-∘ 𝟙))%T.
-  Proof.
-    iApply func_comp_left.
-    - admit.
-    - admit.
-    - iIntros (θ). iApply brel_left_comp.
-   Lemma C_REAL_DH_RAND (f1 f2 : val) (L : sem_row Σ) :
-    sem_val_typed f1 f2 (∀ᵣ θₕ, (((⊤ × (sem_ty_sum 𝟙 𝟙)) -{ θₕ }-> (Option  ⊤)) × ((sem_ty_sum 𝟙 𝟙) -{ θₕ }-> (Option  ⊤))) -{ sem_row_union  θₕ L }-> 𝟙)%T -∗    
-    BREL (REAL_CHAN_DH_REAL f1) ≤ (REAL_CHAN_DH_RAND f2)
-     <|⊥|> {{λ v1 v2,
-                                       ∀ (leakauth1 leakauth2 keyleak1 keyleak2 : label),
-               BREL v1 ((λ: "m", do: leakauth1 (Send "m")), (λ: "m", do: leakauth1 (Recv "m")))%V (λ: "m", do: keyleak1 "m")%V ≤ v2 ((λ: "m", do: leakauth2 (Send "m")), (λ: "m", do: leakauth2 (Recv "m")))%V (λ: "m", do: keyleak2 "m")%V <| (iLblSig_to_iLblThy (envsec_row keyleak1 keyleak2 leakauth1 leakauth2 )) ++ (iLblSig_to_iLblThy L) |> {{ (λ w1 w2, 𝟙%T w1 w2)}}}}.
-   Proof.
-   Admitted.
+  (* Lemma C_REAL_DH_RAND :
+       ⊢ sem_val_typed REAL_CHAN_DH_REAL REAL_CHAN_DH_RAND (∀ᵣ θ__L ,(∀ᵣ θₕ, (((⊤ × (sem_ty_sum 𝟙 𝟙)) -{ θₕ }-> 𝟙) × ((sem_ty_sum 𝟙 𝟙) -{ θₕ }-> (Option  ⊤))) 
+                                                                      -{ sem_row_union  θₕ θ__L }-> 𝟙)
+                                                                ⊸ (∀ᵣ θ₁,∀ᵣ θ2, (((⊤ × (𝟙 + 𝟙)) -{ θ₁ }-> 𝟙) 
+                                                                                    × ((𝟙 + 𝟙) -{ θ₁ }-> Option ⊤)) 
+                                                                                    ⊸ (((⊤ × (𝟙 + 𝟙)) -{ θ2 }-> 𝟙) 
+                                                                                    × ((𝟙 + 𝟙) -{ θ2 }-> Option ⊤)) -{ sem_row_union θ₁ (sem_row_union θ2 θ__L) }-∘ 𝟙))%T.
+     Proof.
+       iApply func_comp_left.
+       - admit.
+       - admit.
+       - iIntros (θ). iApply parallel_comp_right. *)
 
 
   (*F_OAUTH [F_AUTH [C[DH_rand][CHAN[]]]] ≤ F_OAUTH [F_AUTH [C[DH_real][CHAN[]]]]*)
   (*----------------------------------------------------------------------------*)
-  Lemma C_DH_RAND_REAL (f1 f2 : val) (L : sem_row Σ) :
-    sem_val_typed f1 f2 (∀ᵣ θₕ, (((⊤ × (sem_ty_sum 𝟙 𝟙)) -{ θₕ }-> (Option  ⊤)) × ((sem_ty_sum 𝟙 𝟙) -{ θₕ }-> (Option  ⊤))) -{ sem_row_union  θₕ L }-> 𝟙)%T -∗    
-    BREL (REAL_CHAN_DH_RAND f1) ≤ (REAL_CHAN_DH_REAL f2)
-     <|⊥|> {{λ v1 v2,
-                                       ∀ (leakauth1 leakauth2 keyleak1 keyleak2 : label),
-               BREL v1 ((λ: "m", do: leakauth1 (Send "m")), (λ: "m", do: leakauth1 (Recv "m")))%V (λ: "m", do: keyleak1 "m")%V ≤ v2 ((λ: "m", do: leakauth2 (Send "m")), (λ: "m", do: leakauth2 (Recv "m")))%V (λ: "m", do: keyleak2 "m")%V <| (iLblSig_to_iLblThy (envsec_row keyleak1 keyleak2 leakauth1 leakauth2 )) ++ (iLblSig_to_iLblThy L) |> {{ (λ w1 w2, 𝟙%T w1 w2)}}}}.
-  Proof.
-  Admitted.
+  (* Lemma C_DH_RAND_REAL (f1 f2 : val) (L : sem_row Σ) :
+       sem_val_typed f1 f2 (∀ᵣ θₕ, (((⊤ × (sem_ty_sum 𝟙 𝟙)) -{ θₕ }-> (Option  ⊤)) × ((sem_ty_sum 𝟙 𝟙) -{ θₕ }-> (Option  ⊤))) -{ sem_row_union  θₕ L }-> 𝟙)%T -∗    
+       BREL (REAL_CHAN_DH_RAND f1) ≤ (REAL_CHAN_DH_REAL f2)
+        <|⊥|> {{λ v1 v2,
+                                          ∀ (leakauth1 leakauth2 keyleak1 keyleak2 : label),
+                  BREL v1 ((λ: "m", do: leakauth1 (Send "m")), (λ: "m", do: leakauth1 (Recv "m")))%V (λ: "m", do: keyleak1 "m")%V ≤ v2 ((λ: "m", do: leakauth2 (Send "m")), (λ: "m", do: leakauth2 (Recv "m")))%V (λ: "m", do: keyleak2 "m")%V <| (iLblSig_to_iLblThy (envsec_row keyleak1 keyleak2 leakauth1 leakauth2 )) ++ (iLblSig_to_iLblThy L) |> {{ (λ w1 w2, 𝟙%T w1 w2)}}}}.
+     Proof.
+     Admitted. *)
 
   Definition F_AUTH_DH_KE : val :=
     λ: "f",
